\chapter{Algebra}

\section{Polynomial}
Shoeriert multiplication formulas:
$$(x + y)^2 = x^2 + 2xy + y^2$$
$$(x - y)^2 = x^2 - 2xy + y^2$$ 
$$(x + y + z)^2 = x^2 + y^2 + z^2 + 2xy + 2yz + 2zx$$ 
$$(x - y + z)^2 = x^2 + y^2 + z^2 - 2xy - 2yz + 2zx$$ 

Consequences of the above formulas:
$$(-x + y)^2 = (y - x)^2 = y^2 - 2xy + x^2$$
$$(-x - y)^2 = (-(x + y))^2 = (x + y)^2 = x2 + 2xy + y2$$

Formulas for 3rd degree:
$$(x + y)^3 = x^3 + y^3 + 3xy(x + y) = x^3 + 3x^2y + 3xy^2 + y^3$$
$$(x - y)^3 = x^3 - y^3 - 3xy(x - y) = x^3 - 3x^2y + 3xy^2 - y^3$$

Factor Rules:
$$x^2 - y^2 = (x - y)(x + y)$$
$$x^2 + y^2 = (x + y)^2 - 2xy = (x - y)^2 + 2xy$$
$$x^3 - y^3 = (x - y)(x^2 + xy + y^2)$$
$$x^3 + y^3 = (x + y)(x^2 - xy + y^2)$$

More Algebraic Formulas:
$$2(x^2 + y^2) = (x + y)^2 + (x - y)^2$$
$$(x - y)^2 = (x + y)^2 - 4xy$$
$$x^4 + y^4 = (x + y)(x - y)[(x + y)^2 - 2xy]$$

Factoring trinomials:
$$ ax^{2n} + bx^n + c = (ax^n + r)(x^n + \frac{s}{a}) ~~ \text{with} ~ \begin{cases} 
                                                                  r + s = b \\
                                                                  r \times s = ac
                                                                 \end{cases}
$$

Polynomial remainder theorem (the remainder of the division of a polynomial $f(x)$ by a linear polynomial ${(x-a)}$ is equal to $f(a)$:
$$ f(x) = (x-a)q(x) + r(x) \implies f(a) = r(x) $$

Newton's binomial formula:
\[ (x+y)^n = \sum_{k=0}^{n}\binom{n}{k}x^ky^{n-k} \]

\section{Equations}
Quadratic equation solution:
$$ ax^2 + bx + c = 0 \rightarrow (x - x1)(x - x2) = 0 ~\text{with}~ x_{1,2}=\frac{-b\pm\sqrt{b^2-4ac}}{2a}$$

Rational root theorem (or rational root test, rational zero theorem, rational zero test or p/q theorem): 
$$
\text{given } a_nx+^n+...+a_0=0 \rightarrow \text{ solutions are in the form } x=\frac{p}{q} \text{ with } \begin{cases}
p \text{ a factor of } a_0 \\
q \text{ a factor of } a_n
\end{cases}
$$


\section{Inequities TODO}